Use anonymous modules instead of plain kappa (#341)
- Also deprecate CircuitFunctionalEquivalence

silveroak-opentitan/aes/Arrow/sbox_canright_pkg.v
@@ -37,7 +37,7 @@ Open Scope kind_scope.
 (*   return f; *)
 (* endfunction *)
 Definition aes_mul_gf2p2
-  : Kappa << Vector Bit 2, Vector Bit 2, Unit >> << Vector Bit 2 >> :=
+  : << Vector Bit 2, Vector Bit 2, Unit >> ~> << Vector Bit 2 >> :=
 <[ \g d =>
   let a = g[#1] && d[#1] in
   let b = |^g && |^ d in
@@ -46,18 +46,12 @@ Definition aes_mul_gf2p2
 ]>.
 
 Section regression_checks.
-  Notation aes_mul_gf2p2_eval x y :=
-    (bitvec_to_nat (interp_combinational (aes_mul_gf2p2 _) (N2Bv_sized 2 x, (N2Bv_sized 2 y)))).
   Notation aes_mul_gf2p2_test x y o :=
-    (interp_combinational (aes_mul_gf2p2 _) (N2Bv_sized 2 x, (N2Bv_sized 2 y)) = N2Bv_sized 2 o).
+    (kinterp aes_mul_gf2p2 (N2Bv_sized 2 x, (N2Bv_sized 2 y, tt)) = N2Bv_sized 2 o).
 
   Goal aes_mul_gf2p2_test 0 0 0. auto. Qed.
   Goal aes_mul_gf2p2_test 0 1 0. auto. Qed.
   Goal aes_mul_gf2p2_test 2 0 0. auto. Qed.
-  (* Compute aes_mul_gf2p2_eval 0 0. *)
-  (* Compute aes_mul_gf2p2_eval 1 1. *)
-  (* Compute aes_mul_gf2p2_eval 2 2. *)
-  (* Compute aes_mul_gf2p2_eval 3 3. *)
 End regression_checks.
 
 (* // Scale by Omega^2 = N in GF(2^2), using normal basis [Omega^2, Omega] *)
@@ -69,14 +63,12 @@ End regression_checks.
 (*   return d; *)
 (* endfunction *)
 Definition aes_scale_omega2_gf2p2
-  : Kappa << Vector Bit 2, Unit >> << Vector Bit 2 >> :=
+  : << Vector Bit 2, Unit >> ~> << Vector Bit 2 >> :=
 <[ \g => xor g[#1] g[#0] :: g[#0] :: [] ]>.
 
 Section regression_checks.
-  Notation aes_scale_omega2_gf2p2_eval x :=
-    (bitvec_to_nat (interp_combinational (aes_scale_omega2_gf2p2 _) (N2Bv_sized 2 x))).
   Notation aes_scale_omega2_gf2p2_test x o :=
-    (interp_combinational (aes_scale_omega2_gf2p2 _) (N2Bv_sized 2 x) = N2Bv_sized 2 o).
+    (kinterp aes_scale_omega2_gf2p2 (N2Bv_sized 2 x, tt) = N2Bv_sized 2 o).
 
   Goal aes_scale_omega2_gf2p2_test 0 0. auto. Qed.
   Goal aes_scale_omega2_gf2p2_test 1 3. auto. Qed.
@@ -141,7 +133,7 @@ Program Definition aes_mul_gf2p4
 (*   return delta; *)
 (* endfunction *)
 Program Definition aes_square_scale_gf2p4_gf2p2
-  : Kappa << Vector Bit 4, Unit >> << Vector Bit 4>> :=
+  : << Vector Bit 4, Unit >> ~> << Vector Bit 4>> :=
 <[ \gamma =>
     let a = gamma[:3:2] ^ gamma[:1:0] in
     let b = !aes_square_gf2p2 (gamma[:1:0]) in
@@ -163,16 +155,16 @@ parameter logic [7:0] X2A [8] = '{8'h64, 8'h78, 8'h6e, 8'h8c, 8'h68, 8'h29, 8'hd
 parameter logic [7:0] X2S [8] = '{8'h58, 8'h2d, 8'h9e, 8'h0b, 8'hdc, 8'h04, 8'h03, 8'h24};
 parameter logic [7:0] S2X [8] = '{8'h8c, 8'h79, 8'h05, 8'heb, 8'h12, 8'h04, 8'h51, 8'h53}; *)
 
-Definition A2X : Kappa Unit (Vector (Vector Bit 8) 8) := <[ #152:: #243:: #242:: #72:: #9:: #129:: #169:: #255  :: [] ]>.
-Definition X2A : Kappa Unit (Vector (Vector Bit 8) 8) := <[ #100:: #120:: #110:: #140:: #104:: #41:: #222:: #96 :: [] ]>.
-Definition X2S : Kappa Unit (Vector (Vector Bit 8) 8) := <[ #88:: #45:: #158:: #11:: #220:: #4:: #3:: #36       :: [] ]>.
-Definition S2X : Kappa Unit (Vector (Vector Bit 8) 8) := <[ #140:: #121:: #5:: #235:: #18:: #4:: #81:: #83      :: [] ]>.
+Definition A2X : Unit ~> (Vector (Vector Bit 8) 8) := <[ #152:: #243:: #242:: #72:: #9:: #129:: #169:: #255  :: [] ]>.
+Definition X2A : Unit ~> (Vector (Vector Bit 8) 8) := <[ #100:: #120:: #110:: #140:: #104:: #41:: #222:: #96 :: [] ]>.
+Definition X2S : Unit ~> (Vector (Vector Bit 8) 8) := <[ #88:: #45:: #158:: #11:: #220:: #4:: #3:: #36       :: [] ]>.
+Definition S2X : Unit ~> (Vector (Vector Bit 8) 8) := <[ #140:: #121:: #5:: #235:: #18:: #4:: #81:: #83      :: [] ]>.
 
 Section regression_checks.
-  Definition S2X_indexer: Kappa <<Vector Bit 3, Unit>> <<Vector Bit 8>> :=
+  Definition S2X_indexer: <<Vector Bit 3, Unit>> ~> <<Vector Bit 8>> :=
     <[\x => let vec = !S2X in vec[x] ]>.
-  Goal (interp_combinational (S2X_indexer _) (N2Bv_sized 3 2) = N2Bv_sized 8 5).
+  Goal (kinterp S2X_indexer (N2Bv_sized 3 2, tt) = N2Bv_sized 8 5).
   Proof. auto. Qed.
-  Goal (interp_combinational (S2X_indexer _) (N2Bv_sized 3 4) = N2Bv_sized 8 18).
+  Goal (kinterp S2X_indexer (N2Bv_sized 3 4, tt) = N2Bv_sized 8 18).
   Proof. auto. Qed.
 End regression_checks.
